chore(init/algebra/group): use a user attr for transport to additive
This makes it easier to transport more theorems after the original set in this file, without having to restate the map all over again.

library/init/algebra/group.lean
@@ -12,155 +12,7 @@ set_option default_priority 100
 
 set_option old_structure_cmd true
 
-universe u
-variables {α : Type u}
-
-class semigroup (α : Type u) extends has_mul α :=
-(mul_assoc : ∀ a b c : α, a * b * c = a * (b * c))
-
-class comm_semigroup (α : Type u) extends semigroup α :=
-(mul_comm : ∀ a b : α, a * b = b * a)
-
-class left_cancel_semigroup (α : Type u) extends semigroup α :=
-(mul_left_cancel : ∀ a b c : α, a * b = a * c → b = c)
-
-class right_cancel_semigroup (α : Type u) extends semigroup α :=
-(mul_right_cancel : ∀ a b c : α, a * b = c * b → a = c)
-
-class monoid (α : Type u) extends semigroup α, has_one α :=
-(one_mul : ∀ a : α, 1 * a = a) (mul_one : ∀ a : α, a * 1 = a)
-
-class comm_monoid (α : Type u) extends monoid α, comm_semigroup α
-
-class group (α : Type u) extends monoid α, has_inv α :=
-(mul_left_inv : ∀ a : α, a⁻¹ * a = 1)
-
-class comm_group (α : Type u) extends group α, comm_monoid α
-
-@[simp] lemma mul_assoc [semigroup α] : ∀ a b c : α, a * b * c = a * (b * c) :=
-semigroup.mul_assoc
-
-instance semigroup_to_is_associative [semigroup α] : is_associative α (*) :=
-⟨mul_assoc⟩
-
-@[simp] lemma mul_comm [comm_semigroup α] : ∀ a b : α, a * b = b * a :=
-comm_semigroup.mul_comm
-
-instance comm_semigroup_to_is_commutative [comm_semigroup α] : is_commutative α (*) :=
-⟨mul_comm⟩
-
-@[simp] lemma mul_left_comm [comm_semigroup α] : ∀ a b c : α, a * (b * c) = b * (a * c) :=
-left_comm has_mul.mul mul_comm mul_assoc
-
-lemma mul_right_comm [comm_semigroup α] : ∀ a b c : α, a * b * c = a * c * b :=
-right_comm has_mul.mul mul_comm mul_assoc
-
-lemma mul_left_cancel [left_cancel_semigroup α] {a b c : α} : a * b = a * c → b = c :=
-left_cancel_semigroup.mul_left_cancel a b c
-
-lemma mul_right_cancel [right_cancel_semigroup α] {a b c : α} : a * b = c * b → a = c :=
-right_cancel_semigroup.mul_right_cancel a b c
-
-lemma mul_left_cancel_iff [left_cancel_semigroup α] {a b c : α} : a * b = a * c ↔ b = c :=
-⟨mul_left_cancel, congr_arg _⟩
-
-lemma mul_right_cancel_iff [right_cancel_semigroup α] {a b c : α} : b * a = c * a ↔ b = c :=
-⟨mul_right_cancel, congr_arg _⟩
-
-@[simp] lemma one_mul [monoid α] : ∀ a : α, 1 * a = a :=
-monoid.one_mul
-
-@[simp] lemma mul_one [monoid α] : ∀ a : α, a * 1 = a :=
-monoid.mul_one
-
-@[simp] lemma mul_left_inv [group α] : ∀ a : α, a⁻¹ * a = 1 :=
-group.mul_left_inv
-
-def inv_mul_self := @mul_left_inv
-
-@[simp] lemma inv_mul_cancel_left [group α] (a b : α) : a⁻¹ * (a * b) = b :=
-by rw [← mul_assoc, mul_left_inv, one_mul]
-
-@[simp] lemma inv_mul_cancel_right [group α] (a b : α) : a * b⁻¹ * b = a :=
-by simp
-
-@[simp] lemma inv_eq_of_mul_eq_one [group α] {a b : α} (h : a * b = 1) : a⁻¹ = b :=
-by rw [← mul_one a⁻¹, ←h, ←mul_assoc, mul_left_inv, one_mul]
-
-@[simp] lemma one_inv [group α] : 1⁻¹ = (1 : α) :=
-inv_eq_of_mul_eq_one (one_mul 1)
-
-@[simp] lemma inv_inv [group α] (a : α) : (a⁻¹)⁻¹ = a :=
-inv_eq_of_mul_eq_one (mul_left_inv a)
-
-@[simp] lemma mul_right_inv [group α] (a : α) : a * a⁻¹ = 1 :=
-have a⁻¹⁻¹ * a⁻¹ = 1, by rw mul_left_inv,
-by rwa [inv_inv] at this
-
-def mul_inv_self := @mul_right_inv
-
-lemma inv_inj [group α] {a b : α} (h : a⁻¹ = b⁻¹) : a = b :=
-have a = a⁻¹⁻¹, by simp,
-begin rw this, simp [h] end
-
-lemma group.mul_left_cancel [group α] {a b c : α} (h : a * b = a * c) : b = c :=
-have a⁻¹ * (a * b) = b, by simp,
-begin simp [h] at this, rw this end
-
-lemma group.mul_right_cancel [group α] {a b c : α} (h : a * b = c * b) : a = c :=
-have a * b * b⁻¹ = a, by simp,
-begin simp [h] at this, rw this end
-
-instance group.to_left_cancel_semigroup [s : group α] : left_cancel_semigroup α :=
-{ s with mul_left_cancel := @group.mul_left_cancel α s }
-
-instance group.to_right_cancel_semigroup [s : group α] : right_cancel_semigroup α :=
-{ s with mul_right_cancel := @group.mul_right_cancel α s }
-
-lemma mul_inv_cancel_left [group α] (a b : α) : a * (a⁻¹ * b) = b :=
-by rw [← mul_assoc, mul_right_inv, one_mul]
-
-lemma mul_inv_cancel_right [group α] (a b : α) : a * b * b⁻¹ = a :=
-by rw [mul_assoc, mul_right_inv, mul_one]
-
-@[simp] lemma mul_inv_rev [group α] (a b : α) : (a * b)⁻¹ = b⁻¹ * a⁻¹ :=
-inv_eq_of_mul_eq_one begin rw [mul_assoc, ← mul_assoc b, mul_right_inv, one_mul, mul_right_inv] end
-
-lemma eq_inv_of_eq_inv [group α] {a b : α} (h : a = b⁻¹) : b = a⁻¹ :=
-by simp [h]
-
-lemma eq_inv_of_mul_eq_one [group α] {a b : α} (h : a * b = 1) : a = b⁻¹ :=
-have a⁻¹ = b, from inv_eq_of_mul_eq_one h,
-by simp [this.symm]
-
-lemma eq_mul_inv_of_mul_eq [group α] {a b c : α} (h : a * c = b) : a = b * c⁻¹ :=
-by simp [h.symm]
-
-lemma eq_inv_mul_of_mul_eq [group α] {a b c : α} (h : b * a = c) : a = b⁻¹ * c :=
-by simp [h.symm]
-
-lemma inv_mul_eq_of_eq_mul [group α] {a b c : α} (h : b = a * c) : a⁻¹ * b = c :=
-by simp [h]
-
-lemma mul_inv_eq_of_eq_mul [group α] {a b c : α} (h : a = c * b) : a * b⁻¹ = c :=
-by simp [h]
-
-lemma eq_mul_of_mul_inv_eq [group α] {a b c : α} (h : a * c⁻¹ = b) : a = b * c :=
-by simp [h.symm]
-
-lemma eq_mul_of_inv_mul_eq [group α] {a b c : α} (h : b⁻¹ * a = c) : a = b * c :=
-by simp [h.symm, mul_inv_cancel_left]
-
-lemma mul_eq_of_eq_inv_mul [group α] {a b c : α} (h : b = a⁻¹ * c) : a * b = c :=
-by rw [h, mul_inv_cancel_left]
-
-lemma mul_eq_of_eq_mul_inv [group α] {a b c : α} (h : a = c * b⁻¹) : a * b = c :=
-by simp [h]
-
-lemma mul_inv [comm_group α] (a b : α) : (a * b)⁻¹ = a⁻¹ * b⁻¹ :=
-by rw [mul_inv_rev, mul_comm]
-
-/- αdditive "sister" structures.
+/- Additive "sister" structures.
    Example, add_semigroup mirrors semigroup.
    These structures exist just to help automation.
    In an alternative design, we could have the binary operation as an
@@ -181,28 +33,8 @@ by rw [mul_inv_rev, mul_comm]
    to the additive one.
 -/
 
-class add_semigroup (α : Type u) extends has_add α :=
-(add_assoc : ∀ a b c : α, a + b + c = a + (b + c))
-
-class add_comm_semigroup (α : Type u) extends add_semigroup α :=
-(add_comm : ∀ a b : α, a + b = b + a)
-
-class add_left_cancel_semigroup (α : Type u) extends add_semigroup α :=
-(add_left_cancel : ∀ a b c : α, a + b = a + c → b = c)
-
-class add_right_cancel_semigroup (α : Type u) extends add_semigroup α :=
-(add_right_cancel : ∀ a b c : α, a + b = c + b → a = c)
-
-class add_monoid (α : Type u) extends add_semigroup α, has_zero α :=
-(zero_add : ∀ a : α, 0 + a = a) (add_zero : ∀ a : α, a + 0 = a)
-
-class add_comm_monoid (α : Type u) extends add_monoid α, add_comm_semigroup α
-
-class add_group (α : Type u) extends add_monoid α, has_neg α :=
-(add_left_neg : ∀ a : α, -a + a = 0)
-
-class add_comm_group (α : Type u) extends add_group α, add_comm_monoid α
-
+/- Transport multiplicative to additive -/
+section transport
 open tactic
 
 meta def transport_with_dict (dict : name_map name) (src : name) (tgt : name) : command :=
@@ -211,94 +43,274 @@ copy_decl_using dict src tgt
 >> copy_attribute `simp src tt tgt
 >> copy_attribute `instance src tt tgt
 
-/- Transport multiplicative to additive -/
-meta def transport_multiplicative_to_additive (ls : list (name × name)) : command :=
-let dict := native.rb_map.of_list ls in
-ls.foldl (λ t ⟨src, tgt⟩, do
-  env ← get_env,
-  if (env.get tgt).to_bool = ff
-  then t >> transport_with_dict dict src tgt
-  else t)
-skip
+@[user_attribute]
+meta def to_additive_attr : user_attribute (name_map name) name :=
+{ name      := `to_additive,
+  descr     := "Transport multiplicative to additive",
+  cache_cfg := ⟨λ ns, ns.mfoldl (λ dict n, do
+    val ← to_additive_attr.get_param n,
+    pure $ dict.insert n val) mk_name_map, []⟩,
+  parser    := lean.parser.ident,
+  after_set := some $ λ src _ _, do
+    env ← get_env,
+    dict ← to_additive_attr.get_cache,
+    tgt ← to_additive_attr.get_param src,
+    (get_decl tgt >> skip) <|>
+      transport_with_dict dict src tgt }
 
-run_cmd transport_multiplicative_to_additive
-  [/- map operations -/
-   (`has_mul.mul, `has_add.add), (`has_one.one, `has_zero.zero), (`has_inv.inv, `has_neg.neg),
-   (`has_mul, `has_add), (`has_one, `has_zero), (`has_inv, `has_neg),
-   /- map constructors -/
-   (`has_mul.mk, `has_add.mk), (`has_one, `has_zero.mk), (`has_inv, `has_neg.mk),
-   /- map structures -/
-   (`semigroup, `add_semigroup),
-   (`monoid, `add_monoid),
-   (`group, `add_group),
-   (`comm_semigroup, `add_comm_semigroup),
-   (`comm_monoid, `add_comm_monoid),
-   (`comm_group, `add_comm_group),
-   (`left_cancel_semigroup, `add_left_cancel_semigroup),
-   (`right_cancel_semigroup, `add_right_cancel_semigroup),
-   (`left_cancel_semigroup.mk, `add_left_cancel_semigroup.mk),
-   (`right_cancel_semigroup.mk, `add_right_cancel_semigroup.mk),
-   /- map instances -/
-   (`semigroup.to_has_mul, `add_semigroup.to_has_add),
-   (`monoid.to_has_one, `add_monoid.to_has_zero),
-   (`group.to_has_inv, `add_group.to_has_neg),
-   (`comm_semigroup.to_semigroup, `add_comm_semigroup.to_add_semigroup),
-   (`monoid.to_semigroup, `add_monoid.to_add_semigroup),
-   (`comm_monoid.to_monoid, `add_comm_monoid.to_add_monoid),
-   (`comm_monoid.to_comm_semigroup, `add_comm_monoid.to_add_comm_semigroup),
-   (`group.to_monoid, `add_group.to_add_monoid),
-   (`comm_group.to_group, `add_comm_group.to_add_group),
-   (`comm_group.to_comm_monoid, `add_comm_group.to_add_comm_monoid),
-   (`left_cancel_semigroup.to_semigroup, `add_left_cancel_semigroup.to_add_semigroup),
-   (`right_cancel_semigroup.to_semigroup, `add_right_cancel_semigroup.to_add_semigroup),
-   /- map projections -/
-   (`semigroup.mul_assoc, `add_semigroup.add_assoc),
-   (`comm_semigroup.mul_comm, `add_comm_semigroup.add_comm),
-   (`left_cancel_semigroup.mul_left_cancel, `add_left_cancel_semigroup.add_left_cancel),
-   (`right_cancel_semigroup.mul_right_cancel, `add_right_cancel_semigroup.add_right_cancel),
-   (`monoid.one_mul, `add_monoid.zero_add),
-   (`monoid.mul_one, `add_monoid.add_zero),
-   (`group.mul_left_inv, `add_group.add_left_neg),
-   (`group.mul, `add_group.add),
-   (`group.mul_assoc, `add_group.add_assoc),
-   /- map lemmas -/
-   (`mul_assoc, `add_assoc),
-   (`mul_comm, `add_comm),
-   (`mul_left_comm, `add_left_comm),
-   (`mul_right_comm, `add_right_comm),
-   (`one_mul, `zero_add),
-   (`mul_one, `add_zero),
-   (`mul_left_inv, `add_left_neg),
-   (`mul_left_cancel, `add_left_cancel),
-   (`mul_right_cancel, `add_right_cancel),
-   (`mul_left_cancel_iff, `add_left_cancel_iff),
-   (`mul_right_cancel_iff, `add_right_cancel_iff),
-   (`inv_mul_cancel_left, `neg_add_cancel_left),
-   (`inv_mul_cancel_right, `neg_add_cancel_right),
-   (`eq_inv_mul_of_mul_eq, `eq_neg_add_of_add_eq),
-   (`inv_eq_of_mul_eq_one, `neg_eq_of_add_eq_zero),
-   (`inv_inv, `neg_neg),
-   (`mul_right_inv, `add_right_neg),
-   (`mul_inv_cancel_left, `add_neg_cancel_left),
-   (`mul_inv_cancel_right, `add_neg_cancel_right),
-   (`mul_inv_rev, `neg_add_rev),
-   (`mul_inv, `neg_add),
-   (`inv_inj, `neg_inj),
-   (`group.mul_left_cancel, `add_group.add_left_cancel),
-   (`group.mul_right_cancel, `add_group.add_right_cancel),
-   (`group.to_left_cancel_semigroup, `add_group.to_left_cancel_add_semigroup),
-   (`group.to_right_cancel_semigroup, `add_group.to_right_cancel_add_semigroup),
-   (`eq_inv_of_eq_inv, `eq_neg_of_eq_neg),
-   (`eq_inv_of_mul_eq_one, `eq_neg_of_add_eq_zero),
-   (`eq_mul_inv_of_mul_eq, `eq_add_neg_of_add_eq),
-   (`inv_mul_eq_of_eq_mul, `neg_add_eq_of_eq_add),
-   (`mul_inv_eq_of_eq_mul, `add_neg_eq_of_eq_add),
-   (`eq_mul_of_mul_inv_eq, `eq_add_of_add_neg_eq),
-   (`eq_mul_of_inv_mul_eq, `eq_add_of_neg_add_eq),
-   (`mul_eq_of_eq_inv_mul, `add_eq_of_eq_neg_add),
-   (`mul_eq_of_eq_mul_inv, `add_eq_of_eq_add_neg),
-   (`one_inv, `neg_zero)
-]
+end transport
+
+universe u
+variables {α : Type u}
+
+/- map operations -/
+attribute [to_additive has_add.add] has_mul.mul
+attribute [to_additive has_zero.zero] has_one.one
+attribute [to_additive has_neg.neg] has_inv.inv
+attribute [to_additive has_add] has_mul
+attribute [to_additive has_zero] has_one
+attribute [to_additive has_neg] has_inv
+
+/- map constructors -/
+attribute [to_additive has_add.mk] has_mul.mk
+attribute [to_additive has_zero.mk] has_one.mk
+attribute [to_additive has_neg.mk] has_neg.mk
+
+class semigroup (α : Type u) extends has_mul α :=
+(mul_assoc : ∀ a b c : α, a * b * c = a * (b * c))
+class add_semigroup (α : Type u) extends has_add α :=
+(add_assoc : ∀ a b c : α, a + b + c = a + (b + c))
+attribute [to_additive add_semigroup] semigroup
+attribute [to_additive add_semigroup.mk] semigroup.mk
+attribute [to_additive add_semigroup.to_has_add] semigroup.to_has_mul
+attribute [to_additive add_semigroup.add_assoc] semigroup.mul_assoc
+
+class comm_semigroup (α : Type u) extends semigroup α :=
+(mul_comm : ∀ a b : α, a * b = b * a)
+class add_comm_semigroup (α : Type u) extends add_semigroup α :=
+(add_comm : ∀ a b : α, a + b = b + a)
+attribute [to_additive add_comm_semigroup] comm_semigroup
+attribute [to_additive add_comm_semigroup.mk] comm_semigroup.mk
+attribute [to_additive add_comm_semigroup.to_add_semigroup] comm_semigroup.to_semigroup
+attribute [to_additive add_comm_semigroup.add_comm] comm_semigroup.mul_comm
+
+class left_cancel_semigroup (α : Type u) extends semigroup α :=
+(mul_left_cancel : ∀ a b c : α, a * b = a * c → b = c)
+class add_left_cancel_semigroup (α : Type u) extends add_semigroup α :=
+(add_left_cancel : ∀ a b c : α, a + b = a + c → b = c)
+attribute [to_additive add_left_cancel_semigroup] left_cancel_semigroup
+attribute [to_additive add_left_cancel_semigroup.mk] left_cancel_semigroup.mk
+attribute [to_additive add_left_cancel_semigroup.to_add_semigroup] left_cancel_semigroup.to_semigroup
+attribute [to_additive add_left_cancel_semigroup.add_left_cancel] left_cancel_semigroup.mul_left_cancel
+
+class right_cancel_semigroup (α : Type u) extends semigroup α :=
+(mul_right_cancel : ∀ a b c : α, a * b = c * b → a = c)
+class add_right_cancel_semigroup (α : Type u) extends add_semigroup α :=
+(add_right_cancel : ∀ a b c : α, a + b = c + b → a = c)
+attribute [to_additive add_right_cancel_semigroup] right_cancel_semigroup
+attribute [to_additive add_right_cancel_semigroup.mk] right_cancel_semigroup.mk
+attribute [to_additive add_right_cancel_semigroup.to_add_semigroup] right_cancel_semigroup.to_semigroup
+attribute [to_additive add_right_cancel_semigroup.add_right_cancel] right_cancel_semigroup.mul_right_cancel
+
+class monoid (α : Type u) extends semigroup α, has_one α :=
+(one_mul : ∀ a : α, 1 * a = a) (mul_one : ∀ a : α, a * 1 = a)
+class add_monoid (α : Type u) extends add_semigroup α, has_zero α :=
+(zero_add : ∀ a : α, 0 + a = a) (add_zero : ∀ a : α, a + 0 = a)
+attribute [to_additive add_monoid] monoid
+attribute [to_additive add_monoid.mk] monoid.mk
+attribute [to_additive add_monoid.to_has_zero] monoid.to_has_one
+attribute [to_additive add_monoid.to_add_semigroup] monoid.to_semigroup
+attribute [to_additive add_monoid.zero_add] monoid.one_mul
+attribute [to_additive add_monoid.add_zero] monoid.mul_one
+
+class comm_monoid (α : Type u) extends monoid α, comm_semigroup α
+class add_comm_monoid (α : Type u) extends add_monoid α, add_comm_semigroup α
+attribute [to_additive add_comm_monoid] comm_monoid
+attribute [to_additive add_comm_monoid.mk] comm_monoid.mk
+attribute [to_additive add_comm_monoid.to_add_monoid] comm_monoid.to_monoid
+attribute [to_additive add_comm_monoid.to_add_comm_semigroup] comm_monoid.to_comm_semigroup
+
+class group (α : Type u) extends monoid α, has_inv α :=
+(mul_left_inv : ∀ a : α, a⁻¹ * a = 1)
+class add_group (α : Type u) extends add_monoid α, has_neg α :=
+(add_left_neg : ∀ a : α, -a + a = 0)
+attribute [to_additive add_group] group
+attribute [to_additive add_group.mk] group.mk
+attribute [to_additive add_group.to_has_neg] group.to_has_inv
+attribute [to_additive add_group.to_add_monoid] group.to_monoid
+attribute [to_additive add_group.add_left_neg] group.mul_left_inv
+attribute [to_additive add_group.add] group.mul
+attribute [to_additive add_group.add_assoc] group.mul_assoc
+
+class comm_group (α : Type u) extends group α, comm_monoid α
+class add_comm_group (α : Type u) extends add_group α, add_comm_monoid α
+attribute [to_additive add_comm_group] comm_group
+attribute [to_additive add_comm_group.mk] comm_group.mk
+attribute [to_additive add_comm_group.to_add_group] comm_group.to_group
+attribute [to_additive add_comm_group.to_add_comm_monoid] comm_group.to_comm_monoid
+
+@[simp, to_additive add_assoc]
+lemma mul_assoc [semigroup α] : ∀ a b c : α, a * b * c = a * (b * c) :=
+semigroup.mul_assoc
+
+@[to_additive add_semigroup_to_is_associative]
+instance semigroup_to_is_associative [semigroup α] : is_associative α (*) :=
+⟨mul_assoc⟩
+
+@[simp, to_additive add_comm]
+lemma mul_comm [comm_semigroup α] : ∀ a b : α, a * b = b * a :=
+comm_semigroup.mul_comm
+
+@[to_additive add_comm_semigroup_to_is_commutative]
+instance comm_semigroup_to_is_commutative [comm_semigroup α] : is_commutative α (*) :=
+⟨mul_comm⟩
+
+@[simp, to_additive add_left_comm]
+lemma mul_left_comm [comm_semigroup α] : ∀ a b c : α, a * (b * c) = b * (a * c) :=
+left_comm has_mul.mul mul_comm mul_assoc
+
+@[to_additive add_right_comm]
+lemma mul_right_comm [comm_semigroup α] : ∀ a b c : α, a * b * c = a * c * b :=
+right_comm has_mul.mul mul_comm mul_assoc
+
+@[to_additive add_left_cancel]
+lemma mul_left_cancel [left_cancel_semigroup α] {a b c : α} : a * b = a * c → b = c :=
+left_cancel_semigroup.mul_left_cancel a b c
+
+@[to_additive add_right_cancel]
+lemma mul_right_cancel [right_cancel_semigroup α] {a b c : α} : a * b = c * b → a = c :=
+right_cancel_semigroup.mul_right_cancel a b c
+
+@[to_additive add_left_cancel_iff]
+lemma mul_left_cancel_iff [left_cancel_semigroup α] {a b c : α} : a * b = a * c ↔ b = c :=
+⟨mul_left_cancel, congr_arg _⟩
+
+@[to_additive add_right_cancel_iff]
+lemma mul_right_cancel_iff [right_cancel_semigroup α] {a b c : α} : b * a = c * a ↔ b = c :=
+⟨mul_right_cancel, congr_arg _⟩
+
+@[simp, to_additive zero_add]
+lemma one_mul [monoid α] : ∀ a : α, 1 * a = a :=
+monoid.one_mul
+
+@[simp, to_additive add_zero]
+lemma mul_one [monoid α] : ∀ a : α, a * 1 = a :=
+monoid.mul_one
+
+@[simp, to_additive add_left_neg]
+lemma mul_left_inv [group α] : ∀ a : α, a⁻¹ * a = 1 :=
+group.mul_left_inv
+
+@[to_additive neg_add_self]
+def inv_mul_self := @mul_left_inv
+
+@[simp, to_additive neg_add_cancel_left]
+lemma inv_mul_cancel_left [group α] (a b : α) : a⁻¹ * (a * b) = b :=
+by rw [← mul_assoc, mul_left_inv, one_mul]
+
+@[simp, to_additive neg_add_cancel_right]
+lemma inv_mul_cancel_right [group α] (a b : α) : a * b⁻¹ * b = a :=
+by simp
+
+@[simp, to_additive neg_eq_of_add_eq_zero]
+lemma inv_eq_of_mul_eq_one [group α] {a b : α} (h : a * b = 1) : a⁻¹ = b :=
+by rw [← mul_one a⁻¹, ←h, ←mul_assoc, mul_left_inv, one_mul]
+
+@[simp, to_additive neg_zero]
+lemma one_inv [group α] : 1⁻¹ = (1 : α) :=
+inv_eq_of_mul_eq_one (one_mul 1)
+
+@[simp, to_additive neg_neg]
+lemma inv_inv [group α] (a : α) : (a⁻¹)⁻¹ = a :=
+inv_eq_of_mul_eq_one (mul_left_inv a)
+
+@[simp, to_additive add_right_neg]
+lemma mul_right_inv [group α] (a : α) : a * a⁻¹ = 1 :=
+have a⁻¹⁻¹ * a⁻¹ = 1, by rw mul_left_inv,
+by rwa [inv_inv] at this
+
+@[to_additive add_neg_self]
+def mul_inv_self := @mul_right_inv
+
+@[to_additive neg_inj]
+lemma inv_inj [group α] {a b : α} (h : a⁻¹ = b⁻¹) : a = b :=
+have a = a⁻¹⁻¹, by simp,
+begin rw this, simp [h] end
+
+@[to_additive add_group.add_left_cancel]
+lemma group.mul_left_cancel [group α] {a b c : α} (h : a * b = a * c) : b = c :=
+have a⁻¹ * (a * b) = b, by simp,
+begin simp [h] at this, rw this end
+
+@[to_additive add_group.add_right_cancel]
+lemma group.mul_right_cancel [group α] {a b c : α} (h : a * b = c * b) : a = c :=
+have a * b * b⁻¹ = a, by simp,
+begin simp [h] at this, rw this end
+
+@[to_additive add_group.to_left_cancel_add_semigroup]
+instance group.to_left_cancel_semigroup [s : group α] : left_cancel_semigroup α :=
+{ s with mul_left_cancel := @group.mul_left_cancel α s }
+
+@[to_additive add_group.to_right_cancel_add_semigroup]
+instance group.to_right_cancel_semigroup [s : group α] : right_cancel_semigroup α :=
+{ s with mul_right_cancel := @group.mul_right_cancel α s }
+
+@[to_additive add_neg_cancel_left]
+lemma mul_inv_cancel_left [group α] (a b : α) : a * (a⁻¹ * b) = b :=
+by rw [← mul_assoc, mul_right_inv, one_mul]
+
+@[to_additive add_neg_cancel_right]
+lemma mul_inv_cancel_right [group α] (a b : α) : a * b * b⁻¹ = a :=
+by rw [mul_assoc, mul_right_inv, mul_one]
+
+@[simp, to_additive neg_add_rev]
+lemma mul_inv_rev [group α] (a b : α) : (a * b)⁻¹ = b⁻¹ * a⁻¹ :=
+inv_eq_of_mul_eq_one begin rw [mul_assoc, ← mul_assoc b, mul_right_inv, one_mul, mul_right_inv] end
+
+@[to_additive eq_neg_of_eq_neg]
+lemma eq_inv_of_eq_inv [group α] {a b : α} (h : a = b⁻¹) : b = a⁻¹ :=
+by simp [h]
+
+@[to_additive eq_neg_of_add_eq_zero]
+lemma eq_inv_of_mul_eq_one [group α] {a b : α} (h : a * b = 1) : a = b⁻¹ :=
+have a⁻¹ = b, from inv_eq_of_mul_eq_one h,
+by simp [this.symm]
+
+@[to_additive eq_add_neg_of_add_eq]
+lemma eq_mul_inv_of_mul_eq [group α] {a b c : α} (h : a * c = b) : a = b * c⁻¹ :=
+by simp [h.symm]
+
+@[to_additive eq_neg_add_of_add_eq]
+lemma eq_inv_mul_of_mul_eq [group α] {a b c : α} (h : b * a = c) : a = b⁻¹ * c :=
+by simp [h.symm]
+
+@[to_additive neg_add_eq_of_eq_add]
+lemma inv_mul_eq_of_eq_mul [group α] {a b c : α} (h : b = a * c) : a⁻¹ * b = c :=
+by simp [h]
+
+@[to_additive add_neg_eq_of_eq_add]
+lemma mul_inv_eq_of_eq_mul [group α] {a b c : α} (h : a = c * b) : a * b⁻¹ = c :=
+by simp [h]
+
+@[to_additive eq_add_of_add_neg_eq]
+lemma eq_mul_of_mul_inv_eq [group α] {a b c : α} (h : a * c⁻¹ = b) : a = b * c :=
+by simp [h.symm]
+
+@[to_additive eq_add_of_neg_add_eq]
+lemma eq_mul_of_inv_mul_eq [group α] {a b c : α} (h : b⁻¹ * a = c) : a = b * c :=
+by simp [h.symm, mul_inv_cancel_left]
+
+@[to_additive add_eq_of_eq_neg_add]
+lemma mul_eq_of_eq_inv_mul [group α] {a b c : α} (h : b = a⁻¹ * c) : a * b = c :=
+by rw [h, mul_inv_cancel_left]
+
+@[to_additive add_eq_of_eq_add_neg]
+lemma mul_eq_of_eq_mul_inv [group α] {a b c : α} (h : a = c * b⁻¹) : a * b = c :=
+by simp [h]
+
+@[to_additive neg_add]
+lemma mul_inv [comm_group α] (a b : α) : (a * b)⁻¹ = a⁻¹ * b⁻¹ :=
+by rw [mul_inv_rev, mul_comm]
 
 instance add_semigroup_to_is_eq_associative [add_semigroup α] : is_associative α (+) :=
 ⟨add_assoc⟩
@@ -306,8 +318,6 @@ instance add_semigroup_to_is_eq_associative [add_semigroup α] : is_associative 
 instance add_comm_semigroup_to_is_eq_commutative [add_comm_semigroup α] : is_commutative α (+) :=
 ⟨add_comm⟩
 
-def neg_add_self := @add_left_neg
-def add_neg_self := @add_right_neg
 def eq_of_add_eq_add_left := @add_left_cancel
 def eq_of_add_eq_add_right := @add_right_cancel
 
